ADD instruction

src/Dafny/llvm.i.dfy
@@ -11,15 +11,11 @@ module LLVM_def {
     type LocalVar = string
     type GlobalVar = string
 
-    datatype Value = uint8 | uint16 | uint32 | uint64 | uint128
-
-
     datatype state = State(
         lvs:map<LocalVar, Value>,
         gvs:map<GlobalVar, Value>,
         m:memmap,
         ok:bool)
-
 
     // Taken from Vale -- modify for llvm
     type shift_amount = s | 0 <= s < 32 // Some shifts allow s=32, but we'll be conservative for simplicity
@@ -28,13 +24,8 @@ module LLVM_def {
         | LSRShift(amount_lsr:shift_amount)
         | RORShift(amount_ror:shift_amount)
 
-    // datatype operand = OConst(n:uint32)
-        // | OReg(r:addr)
-        // | OShift(reg:addr, s:Shift)
-        // | OSymbol(sym:GlobalVar)
-        // | OSP
-        // | OLR
-    datatype operand = Value | LocalVar | GlobalVar
+
+    datatype operand = Val(v:Value) | LV(l:LocalVar) | GV(g:GlobalVar)
 
     //---
     //-----------------------------------------------------------------------------
@@ -42,7 +33,7 @@ module LLVM_def {
     //-----------------------------------------------------------------------------
 
     datatype ins =
-    | ADD(t:Value, src1ADD:operand, src2ADD:operand)
+    | ADD(dst:operand, src1ADD:operand, src2ADD:operand)
     | SUB(t:Value, src1ADD:operand, src2ADD:operand)
     | BR(cond:bool, labelTrue:string,labelFalse:string)
     | CALL() //needs work
@@ -75,17 +66,19 @@ module LLVM_def {
         ValidRegState(s.lvs,s.gvs) && ValidMemState(s.m)
     }
 
-    predicate ValidOperand(o:operand)
+    predicate ValidOperand(s:state,o:operand)
     {
         match o
-            case Value => true
-            case LocalVar => true
-            case GlobalVar => true
+            case Val(v) => true
+            case LV(l) => l in s.lvs
+            case GV(g) => g in s.gvs
     }
+
     predicate ValidInstruction(s:state, ins:ins)
     {
         ValidState(s) && match ins
-            case ADD(t,src1,src2) => ValidOperand(src1) && ValidOperand(src2)
+            case ADD(t,src1,src2) => ValidOperand(s,t) && ValidOperand(s,src1) && ValidOperand(s,src2) 
+                                    && matchOps(OperandContents(s,t),OperandContents(s,src1),OperandContents(s,src2))
             case SUB(t,src1,src2) => true
             case BR(cond, labelTrue,labelFalse) => true
             case CALL() => true
@@ -99,23 +92,77 @@ module LLVM_def {
                  
     }
 
+    predicate matchOps(v0:Value,v1:Value,v2:Value)
+    {
+        (v0.Val8? ==> v1.Val8? && v2.Val8?)
+        && (v0.Val16? ==> v1.Val16? && v2.Val16?)
+        && (v0.Val32? ==> v1.Val32? && v2.Val32?)
+        && (v0.Val64? ==> v1.Val64? && v2.Val64?)
+        && (v0.Val128? ==> v1.Val128? && v2.Val128?)
+    }
     //EVAL//
-    predicate ValidRegOperand(o:operand)
+    predicate ValidRegOperand(s:state, o:operand)
     { 
-        // !o.OConst? && !o.OShift? && ValidOperand(o) 
-        ValidOperand(o)
+        ValidOperand(s,o)
     }
 
-    predicate evalUpdate(s:state, o:operand, v:uint32, r:state)
+    function OperandContents(s:state, o:operand): Value
+        requires ValidOperand(s,o)
         requires ValidState(s)
-        requires ValidRegOperand(o)
-        ensures evalUpdate(s, o, v, r) ==> ValidState(r)
+    {
+        // let x:Value | 0;
+
+        reveal_ValidRegState();
+        match o
+            case Val(v) => v
+            case LV(l) => s.lvs[l]
+            case GV(g) => s.gvs[g]
+           
+    }
+
+
+    predicate evalUpdate(s:state, o:operand, val:Value, r:state)
+        requires ValidState(s)
+        requires ValidRegOperand(s,o)
+        ensures evalUpdate(s, o, val, r) ==> ValidState(r)
     {
         reveal_ValidRegState();
         match o
-            case Value => r == s 
-            case LocalVar => r == s 
-            case GlobalVar => r == s 
+            case Val(v) => r == s 
+            case GV(g) => r == s.(gvs := s.gvs[g := val]) 
+            case LV(l) => r == s.(lvs := s.lvs[l := val]) 
+            
+    }
+
+    predicate evalIns(ins:ins, s:state, r:state)
+    {   
+        if !s.ok || !ValidInstruction(s, ins) then !r.ok
+        else match ins
+            case ADD(t,src1,src2) => evalUpdate(s, t, 
+                                evalADD(OperandContents(s,t),OperandContents(s,src1),OperandContents(s,src2)),r)
+            case SUB(t,src1,src2) => true
+            case BR(cond, labelTrue,labelFalse) => true
+            case CALL() => true
+            case GETELEMENTPTR(t,p) => true
+            case ICMP() => true
+            case RET() => true
+            case SEXT() => true
+            case SHL() => true
+            case TRUN() => true
+            case ZEXT() => true
+    }
+
+
+
+
+    function evalADD(v0:Value,v1:Value,v2:Value): Value
+        requires matchOps(v0,v1,v2)
+    {
+       if v0.Val8? then Val8(BitwiseAdd8(ValueContents8Bit(v1),ValueContents8Bit(v2))) else 
+       if v0.Val16? then Val16(BitwiseAdd16(ValueContents16Bit(v1),ValueContents16Bit(v2))) else
+       if v0.Val32? then Val32(BitwiseAdd32(ValueContents32Bit(v1),ValueContents32Bit(v2))) else
+       if v0.Val64? then Val64(BitwiseAdd64(ValueContents64Bit(v1),ValueContents64Bit(v2))) else
+                        Val128(BitwiseAdd128(ValueContents128Bit(v1),ValueContents128Bit(v2)))
     }
 
 }
